find min repro

btree.dfy
@@ -6,123 +6,229 @@ datatype LeafCell<T> = LeafCell(key: Key, value: T)
 datatype InnerCell = InnerCell(key: Key, child: PageNumber)
 datatype Cell<T> = Cell(key: Key, value: T)
 
-class Span<T>
-{
-    var Array: array<T>;
-    var Offset: int;
-    var Count: int;
+newtype {:nativeType "uint"} u32 = x | 0 <= x < 0x1_0000_0000
+newtype {:nativeType "ulong"} u64 = x | 0 <= x < 0x1_0000_0000_0000_0000
 
-    function Valid() : bool 
+class Vector<T>
+{
+    var cells: array?<T>;
+    var used: u64;
+
+    constructor ()
+        ensures Valid()
+        ensures this.used == 0
+        ensures this.cells == null
+    {
+        this.used := 0;
+        this.cells := null;
+    }
+
+    function Valid() : bool
         reads this
     {
-        (0 <= Offset < Array.Length) &&
-        (0 <= Count < Array.Length) &&
-        (Offset + Count <= Array.Length)
+        if this.cells == null then 
+            this.used == 0
+        else (
+            (0 < this.cells.Length < 0x1_0000_0000_0000_0000) &&
+            (0 <= used <= cells.Length as u64)
+        )
     }
 
-    // function method LastIndex() : (i: int)
-    //     requires Valid()
-    //     requires Count > 0
-    //     reads this
-    //     ensures i == (Offset + Count - 1)
-    // {
-    //     Offset + Count - 1
-    // }
-
-    function before() : (s: seq<T>)
+    method try_pop() returns (value: Option<T>)
         requires Valid()
-        reads this, this.Array
+        modifies this, this.cells
+        ensures Valid()
+        ensures if old(this.used) > 0 then (
+            (this.used == (old(this.used) - 1)) &&
+            (value == Some(old(this.cells[this.used-1])))
+        ) else (
+            (this.used == old(this.used)) &&
+            (value == None)
+        )
     {
-        Array[..Offset]
+        if (this.cells != null && this.used > 0) {
+            this.used := this.used - 1;
+            return Some(this.cells[this.used]);
+        } else {
+            return None;
+        }
     }
 
-    function after() : (s: seq<T>)
+    method push(value: T)
         requires Valid()
-        reads this, this.Array
+        requires this.used < 0xFFFF_FFFF_FFFF_FFFF
+        modifies this, this.cells
+        ensures Valid()
+        ensures this.cells != null
+        ensures old(this.used) + 1 == this.used
+        ensures old(this.cells == null) || old(this.cells[..this.used]) == this.cells[..(this.used-1)]
+        ensures this.cells[this.used - 1] == value
+        //ensures old(this.cells == null) || old(this.used == this.cells.Length as u64) || old(this.cells[this.used+1..]) == this.cells[this.used..]
     {
-        Array[Offset+Count..]
+        if (cells == null || used == cells.Length as u64)
+        {
+            var len: u64 := 
+                if cells == null 
+                then 0 as u64
+                else this.cells.Length as u64;
+
+            var newLen: u64;
+            if (len == 0) {
+                newLen := 1;
+            } else if (len < 0x8000_0000_0000_0000 as u64) {
+                newLen := len * 2;
+            } else {
+                newLen := 0xFFFF_FFFF_FFFF_FFFF as u64;
+            }
+
+            var a := new T[newLen]((ii: int) reads this,cells => (
+                assume 0 <= ii < newLen as int;
+                var i: u64 := ii as u64;
+                assume cells == null || len as int == cells.Length;
+                if cells == null then
+                    value
+                else if 0 <= i < len then
+                    cells[i]
+                else
+                    value
+            ));
+
+            this.cells := a;
+        }
+
+        this.cells[used] := value;
+        used := used + 1 as u64;
     }
 
-    function method sequence() : (s: seq<T>)
+    function sequence() : (s: seq<T>)
         requires Valid()
-        reads this, this.Array
+        reads this, this.cells
     {
-        Array[Offset..Offset+Count]
+        if this.cells == null then [] else this.cells[..this.used]
     }
-
-    function method get(idx: int) : (v: T)
-        requires Valid()
-        requires 0 <= idx < Count
-        reads this, this.Array
-        ensures this.Array[Offset+idx] == v
-    {
-        Array[Offset+idx]
-    }
-
-    method put(idx: int, v: T)
-        requires Valid()
-        requires 0 <= idx < Count
-        modifies this.Array
-        ensures old(Array.Length) == Array.Length
-        ensures old(before()) == before()
-        ensures old(sequence()[..idx]) == sequence()[..idx]
-        ensures v == sequence()[idx]
-        ensures old(sequence()[idx+1..]) == sequence()[idx+1..]
-        ensures old(after()) == after()
-    {
-        Array[Offset+idx] := v;
-    }
-
 }
 
-method rotate_one<T>(s: Span<T>)
-    requires s.Valid()
-    requires s.Count > 1
-    modifies s.Array
-    ensures old(s.Array.Length) == s.Array.Length
-    ensures old(s.before()) == s.before()
-    ensures old(s.sequence()[..(s.Count-1)]) == s.sequence()[1..]
-    ensures old(s.sequence()[s.Count-1]) == s.sequence()[0]
-    ensures old(s.after()) == s.after()
+method vector_test() 
 {
-    ghost var orig := s.sequence();
+    var v := new Vector<int>();
 
-    var wrapped := s.Array[s.Offset+s.Count-1];
+    assert [] == v.sequence();
 
-    var doneIdx := s.Count;
-    while doneIdx > 1 
-        decreases doneIdx
-        invariant old(s.before()) == s.before()
-        invariant old(s.after()) == s.after()
-        invariant 1 <= doneIdx <= s.Count
-        invariant orig[..doneIdx] == s.sequence()[..doneIdx]
-        invariant orig[(doneIdx-1)..s.Count-1] == s.sequence()[doneIdx..s.Count]
-    {
-        assert orig[(doneIdx-1)..s.Count-1] == s.sequence()[doneIdx..s.Count];
-        doneIdx := doneIdx - 1;
-        assert orig[doneIdx..s.Count-1] == s.sequence()[(doneIdx+1)..s.Count];
-        ghost var x := s.sequence();
-        s.put(doneIdx, s.get(doneIdx-1));
-        assert orig[doneIdx..s.Count-1] == s.sequence()[(doneIdx+1)..s.Count];
-        assert orig[(doneIdx-1)] == s.sequence()[doneIdx-1];
-        assert orig[(doneIdx-1)] == s.sequence()[doneIdx];
-        assert |orig[(doneIdx-1)..s.Count-1]| == |s.sequence()[doneIdx..s.Count]|;
-        assert orig[(doneIdx-1)..s.Count-1] == s.sequence()[doneIdx..s.Count];
-    }
+    var i: Option<int>;
+    i := v.try_pop();
+    assert i == None;
 
-    assert |orig[..(s.Count-1)]| == |s.sequence()[1..]|;
-    assert orig[..(s.Count-1)] == s.sequence()[1..];
+    v.push(1);
+    assert [1] == v.sequence();
 
-    s.Array[s.Offset] := wrapped;
+    // i := v.try_pop();
+    // assert Some(1) == i;
 }
 
-// method insert_at<T>(cells: array<T>, idx: int, value: T)
-//     requires 0 <= idx < cells.Length
-//     modifies cells
-//     ensures old(cells.Length) == cells.Length
-//     ensures old(cells[..idx]) == cells[..idx]
-//     ensures cells[idx] == value
-//     ensures old(cells[idx..(cells.Length-1)]) == cells[(idx+1)..]
+// class Span<T>
+// {
+//     var Array: array<T>;
+//     var Offset: int;
+//     var Count: int;
+
+//     function Valid() : bool 
+//         reads this
+//     {
+//         (0 <= Offset < Array.Length) &&
+//         (0 <= Count < Array.Length) &&
+//         (Offset + Count <= Array.Length)
+//     }
+
+//     function before() : (s: seq<T>)
+//         requires Valid()
+//         reads this, this.Array
+//     {
+//         Array[..Offset]
+//     }
+
+//     function after() : (s: seq<T>)
+//         requires Valid()
+//         reads this, this.Array
+//     {
+//         Array[Offset+Count..]
+//     }
+
+//     function method sequence() : (s: seq<T>)
+//         requires Valid()
+//         reads this, this.Array
+//     {
+//         Array[Offset..Offset+Count]
+//     }
+
+//     function method get(idx: int) : (v: T)
+//         requires Valid()
+//         requires 0 <= idx < Count
+//         reads this, this.Array
+//         ensures this.Array[Offset+idx] == v
+//     {
+//         Array[Offset+idx]
+//     }
+
+//     method put(idx: int, v: T)
+//         requires Valid()
+//         requires 0 <= idx < Count
+//         modifies this.Array
+//         ensures old(Array.Length) == Array.Length
+//         ensures old(before()) == before()
+//         ensures old(sequence()[..idx]) == sequence()[..idx]
+//         ensures v == sequence()[idx]
+//         ensures old(sequence()[idx+1..]) == sequence()[idx+1..]
+//         ensures old(after()) == after()
+//     {
+//         Array[Offset+idx] := v;
+//     }
+
+// }
+
+// method push_front<T>(s: Span<T>, v: T)
+//     requires s.Valid()
+//     requires s.Count > 1
+//     modifies s.Array
+//     ensures old(s.Count) + 1 == s.Count
+//     ensures old(s.before()) == s.before()
+//     ensures v == s.sequence()[0]
+//     ensures old(s.sequence()[..]) == s.sequence()[1..]
+//     ensures old(s.after()) == s.after()
+// {
+//     ghost var orig := s.sequence();
+
+
+//     var doneIdx := s.Count;
+//     while doneIdx > 1 
+//         decreases doneIdx
+//         invariant old(s.before()) == s.before()
+//         invariant old(s.after()) == s.after()
+//         invariant 1 <= doneIdx <= s.Count
+//         invariant orig[..doneIdx] == s.sequence()[..doneIdx]
+//         invariant orig[(doneIdx-1)..s.Count-1] == s.sequence()[doneIdx..s.Count]
+//     {
+//         assert orig[(doneIdx-1)..s.Count-1] == s.sequence()[doneIdx..s.Count];
+//         doneIdx := doneIdx - 1;
+//         assert orig[doneIdx..s.Count-1] == s.sequence()[(doneIdx+1)..s.Count];
+//         ghost var x := s.sequence();
+//         s.put(doneIdx, s.get(doneIdx-1));
+//         assert orig[doneIdx..s.Count-1] == s.sequence()[(doneIdx+1)..s.Count];
+//         assert orig[(doneIdx-1)] == s.sequence()[doneIdx-1];
+//         assert orig[(doneIdx-1)] == s.sequence()[doneIdx];
+//         assert |orig[(doneIdx-1)..s.Count-1]| == |s.sequence()[doneIdx..s.Count]|;
+//         assert orig[(doneIdx-1)..s.Count-1] == s.sequence()[doneIdx..s.Count];
+//     }
+
+//     assert |orig[..(s.Count-1)]| == |s.sequence()[1..]|;
+//     assert orig[..(s.Count-1)] == s.sequence()[1..];
+// }
+
+// method insert_at<T>(cells: Span<T>, idx: int, value: T)
+//     requires 0 <= idx < cells.Count
+//     modifies cells.Array
+//     ensures old(cells.before()) == cells.before()
+//     ensures cells.get(idx) == value
+//     ensures old(cells.after()) == cells.after()
 // {
 //     ghost var orig := cells[..];
 
